theories/L7/L6_to_Clight.v
@@ -1162,8 +1162,9 @@ Fixpoint make_funinfo
         add_bodyinfo e' fenv nenv' map defs
       end
   | _ => ret None
-  end.
+  end. 
 
+Definition retVoid : rettype := compcert.common.AST.Tvoid.
 
 Definition global_defs (e : exp)
            : list (positive * globdef Clight.fundef type) :=
@@ -1176,13 +1177,13 @@ Definition global_defs (e : exp)
     :: *)
   (gcIdent,
    Gfun (External (EF_external "gc"
-                  (mksignature (val_typ :: nil) None cc_default))
+                  (mksignature (val_typ :: nil) retVoid cc_default))
       (Tcons (Tpointer val noattr) (Tcons threadInf Tnil))
       Tvoid
       cc_default)) ::
   (isptrIdent,
    Gfun (External (EF_external "is_ptr"
-                             (mksignature (val_typ :: nil) None cc_default))
+                             (mksignature (val_typ :: nil) retVoid cc_default))
       (Tcons val Tnil) (Tint IBool Unsigned noattr)
       cc_default)) ::
   nil.
@@ -1545,7 +1546,7 @@ Definition exportIdent := 21%positive.
 Definition make_tinfo_rec : positive * globdef Clight.fundef type :=
   (make_tinfoIdent,
    Gfun (External (EF_external "make_tinfo"
-                               (mksignature (nil) (Some val_typ) cc_default))
+                               (mksignature (nil) (Tret val_typ) cc_default))
                   Tnil
                   threadInf
                   cc_default)).
@@ -1553,7 +1554,7 @@ Definition make_tinfo_rec : positive * globdef Clight.fundef type :=
 Definition export_rec : positive * globdef Clight.fundef type :=
   (exportIdent,
    Gfun (External (EF_external "export"
-                               (mksignature (cons val_typ nil) (Some val_typ) cc_default))
+                               (mksignature (cons val_typ nil) (Tret val_typ) cc_default))
                   (Tcons threadInf Tnil)
                   valPtr
                   cc_default)).
@@ -1709,7 +1710,7 @@ Definition make_header
 
 
 (* end of header file *)
-Require Import L6.cps_show.
+
 
 Definition compile (e : exp) (cenv : ctor_env) (nenv : M.t BasicAst.name) :
   exceptionMonad.exception (M.t BasicAst.name * option Clight.program * option Clight.program) :=
