theories/L7/L6_to_Clight_stack.v
@@ -1123,6 +1123,7 @@ Fixpoint make_funinfo (e : exp) (fenv : fun_env) (nenv : name_env)
   | _ => failwith "make_funinfo: Function block expected"
   end.
 
+Definition retVoid : rettype := compcert.common.AST.Tvoid.
 
 Definition global_defs (e : exp)
   : list (positive * globdef Clight.fundef type) :=
@@ -1134,13 +1135,13 @@ Definition global_defs (e : exp)
                                     false false))
     :: *)
     (gcIdent , Gfun (External (EF_external "gc"
-                                              (mksignature (val_typ :: nil) None cc_default))
+                                              (mksignature (val_typ :: nil) retVoid cc_default))
                                  (Tcons (Tpointer val noattr) (Tcons threadInf Tnil))
                                  Tvoid
                                  cc_default
     ))::
       (isptrIdent , Gfun (External (EF_external "is_ptr"
-                                             (mksignature (val_typ :: nil) None cc_default))
+                                             (mksignature (val_typ :: nil) retVoid cc_default))
                                 (Tcons val Tnil) (Tint IBool Unsigned noattr)
                                 cc_default
       ))
@@ -1480,7 +1481,7 @@ Definition exportIdent := 21%positive.
 Definition make_tinfo_rec : positive * globdef Clight.fundef type :=
   (make_tinfoIdent,
    Gfun (External (EF_external "make_tinfo"
-                               (mksignature (nil) (Some val_typ) cc_default))
+                               (mksignature (nil) (Tret val_typ) cc_default))
                   Tnil
                   threadInf
                   cc_default)).
@@ -1488,7 +1489,7 @@ Definition make_tinfo_rec : positive * globdef Clight.fundef type :=
 Definition export_rec : positive * globdef Clight.fundef type :=
   (exportIdent,
    Gfun (External (EF_external "export"
-                               (mksignature (cons val_typ nil) (Some val_typ) cc_default))
+                               (mksignature (cons val_typ nil) (Tret val_typ) cc_default))
                   (Tcons threadInf Tnil)
                   valPtr
                   cc_default)).
